new semantics with anon

LambdaSemantics.v
@@ -23,39 +23,24 @@ Open Scope string_scope.
 (* ---------------------------------------------------------------------- *)
 (** Representation of variables *)
 
-Definition name := string.
+Definition var := string.
 
-Inductive var : Type :=
-  | var_anon : var
-  | var_name : name -> var.
+Inductive bind : Type :=
+  | bind_anon : bind
+  | bind_var : var -> bind.
 
-Definition eq_name_dec := String.string_dec.
+Definition eq_var_dec := String.string_dec.
 
-Definition name_eq (s1 s2:name) : bool :=
-  if eq_name_dec s1 s2 then true else false.
+Definition var_eq (s1:var) (s2:var) : bool :=
+  if eq_var_dec s1 s2 then true else false.
 
-Lemma name_eq_spec : forall s1 s2,
-  name_eq s1 s2 = isTrue (s1 = s2).
+Lemma var_eq_spec : forall s1 s2,
+  var_eq s1 s2 = isTrue (s1 = s2).
 Proof using.
-  intros. unfold name_eq. case_if; rew_bool_eq~.
+  intros. unfold var_eq. case_if; rew_bool_eq~.
 Qed.
 
-Definition var_eq (x1 x2:var) : bool :=
-  match x1, x2 with
-  | var_anon, var_anon => true
-  | var_name s1, var_name s2 => name_eq s1 s2
-  | _, _ => false
-  end.
-
-Lemma var_eq_spec : forall x1 x2,
-  var_eq x1 x2 = isTrue (x1 = x2).
-Proof using.
-  intros. unfold var_eq. destruct x1; destruct x2; 
-   try rewrite name_eq_spec; rew_bool_eq; auto_false*.
-  { iff; congruence. } (* LATER:simplify*)
-Qed.
-
-Global Opaque name.
+Global Opaque var.
 
 
 (* ---------------------------------------------------------------------- *)
@@ -89,14 +74,14 @@ Inductive val : Type :=
   | val_int : int -> val
   | val_loc : loc -> val
   | val_prim : prim -> val
-  | val_fix : var -> var -> trm -> val
+  | val_fix : bind -> bind -> trm -> val
 
 with trm : Type :=
   | trm_val : val -> trm
   | trm_var : var -> trm
-  | trm_fix : var -> var -> trm -> trm
+  | trm_fix : bind -> bind -> trm -> trm
   | trm_if : trm -> trm -> trm -> trm
-  | trm_let : var -> trm -> trm -> trm
+  | trm_let : bind -> trm -> trm -> trm
   | trm_app : trm -> trm -> trm
   | trm_while : trm -> trm -> trm
   | trm_for : var -> trm -> trm -> trm -> trm.
@@ -108,24 +93,13 @@ Proof using. apply (Inhab_of_val val_unit). Qed.
 
 (** Encoded constructs *)
 
-(*
-Definition trm_seq (t1:trm) (t2:trm) :=
-  trm_let var_anon t1 t2.
-
-Definition trm_fun (x:var) (t1:trm) :=
-  trm_fix var_anon x t1.
-
-Definition val_fun (x:var) (t1:trm) :=
-  val_fix var_anon x t1.
-*)
-
-Notation "'trm_seq' t1 t2" := (trm_let var_anon t1 t2) 
+Notation "'trm_seq' t1 t2" := (trm_let bind_anon t1 t2)
   (at level 69, t1 at level 0, t2 at level 0).
 
-Notation "'trm_fun' x t1" := (trm_fix var_anon x t1) 
+Notation "'trm_fun' x t1" := (trm_fix bind_anon x t1)
   (at level 69, x at level 0, t1 at level 0).
 
-Notation "'val_fun' x t1" := (val_fix var_anon x t1) 
+Notation "'val_fun' x t1" := (val_fix bind_anon x t1)
   (at level 69, x at level 0, t1 at level 0).
 
 
@@ -139,55 +113,112 @@ Coercion val_loc : loc >-> val.
 Coercion trm_val : val >-> trm.
 Coercion trm_var : var >-> trm.
 Coercion trm_app : trm >-> Funclass.
-Coercion var_name : name >-> var.
+Coercion bind_var : var >-> bind.
 
 
 (* ********************************************************************** *)
 (* * Source language semantics *)
 
 (* ---------------------------------------------------------------------- *)
-(** Definition of capture-avoiding substitution *)
+(** Definition of contexts *)
 
-Definition var_match (x1:var) (x2:var) : bool :=
-  match x1,x2 with
-  | var_name s1, var_name s2 => name_eq s1 s2
-  | _,_ => false
+(** [ctx] describes a list of bindings *)
+
+Definition ctx : Type :=
+  list (var * val).
+
+(** [ctx_empty] describes the empty context *)
+
+Definition ctx_empty : ctx :=
+  nil.
+
+(** [ctx_add z v E] is defined as:
+    - [E] if [z] is the anonymous binder
+    - [E] extended with the pair [(x,v)] if [z] is a variable [x]. *)
+
+Definition ctx_add (z:bind) (v:val) (E:ctx) : ctx :=
+  match z with
+  | bind_anon => E
+  | bind_var x => (x,v)::E
   end.
 
-Fixpoint subst (y:var) (w:val) (t:trm) : trm :=
-  let aux t := subst y w t in
-  let aux_no_capture x t := if var_match x y then t else aux t in
-  match t with
-  | trm_val v => trm_val v
-  | trm_var x => if var_match x y then trm_val w else t
-  | trm_fix f x t1 => trm_fix f x (if var_match f y then t1 else
-                                   aux_no_capture x t1)
-  | trm_if t0 t1 t2 => trm_if (aux t0) (aux t1) (aux t2)
-  | trm_let x t1 t2 => trm_let x (aux t1) (aux_no_capture x t2)
-  | trm_app t1 t2 => trm_app (aux t1) (aux t2)
-  | trm_while t1 t2 => trm_while (aux t1) (aux t2)
-  | trm_for x t1 t2 t3 => trm_for x (aux t1) (aux t2) (aux_no_capture x t3)
+(** [ctx_one z v] is a shorthand for [ctx_add z v ctx_empty] *)
+
+Definition ctx_one (z:bind) (v:val) : ctx :=
+  ctx_add z v ctx_empty.
+
+(** [ctx_two z1 v1 z2 v2] is a shorthand for
+    [ctx_add z1 v1 (ctx_add z2 v2 ctx_empty)]. *)
+
+Definition ctx_two (z1:bind) (v1:val) (z2:bind) (v2:val) : ctx :=
+  ctx_add z1 v1 (ctx_add z2 v2 ctx_empty).
+
+(** [ctx_rem x E] removes all bindings on [x] stored in [E] *)
+
+Fixpoint ctx_rem_var (x:var) (E:ctx) : ctx :=
+  match E with
+  | nil => nil
+  | (y,v)::E' =>
+      let E'' := ctx_rem_var x E' in
+      if var_eq x y then E'' else (y,v)::E''
   end.
+
+Fixpoint ctx_rem (z:bind) (E:ctx) : ctx :=
+  match z with
+  | bind_anon => E
+  | bind_var x => ctx_rem_var x E
+  end.
+
+(** [ctx_lookup x E] returns
+    - [None] if [x] is not bound in [E]
+    - [Some v] if [x] is bound to [v] in [E]. *)
+
+Fixpoint ctx_lookup (x:var) (E:ctx) : option val :=
+  match E with
+  | nil => None
+  | (y,v)::E' => if var_eq x y
+                   then Some v
+                   else ctx_lookup x E'
+  end.
+
+(** [ctx_fresh x E] asserts that [x] is not bound in [E] *)
+
+Definition ctx_fresh (x:var) (E:ctx) : Prop :=
+  ctx_lookup x E = None.
 
 
 (* ---------------------------------------------------------------------- *)
-(** Characterization of values *)
+(** Definition of capture-avoiding substitution *)
 
-Definition trm_is_val (t:trm) : Prop :=
+(** [subst E t] substitutes all the bindings from [E] inside [t] *)
+
+Fixpoint subst (E:ctx) (t:trm) : trm :=
+  let aux := subst E in
   match t with
-  | trm_val v => True
-  | _ => False
+  | trm_val v => trm_val v
+  | trm_var x => match ctx_lookup x E with
+                 | None => t
+                 | Some v => v
+                 end
+  | trm_fix f z t1 => trm_fix f z (subst (ctx_rem z (ctx_rem f E)) t1)
+  | trm_if t0 t1 t2 => trm_if (aux t0) (aux t1) (aux t2)
+  | trm_let z t1 t2 => trm_let z (aux t1) (subst (ctx_rem z E) t2)
+  | trm_app t1 t2 => trm_app (aux t1) (aux t2)
+  | trm_while t1 t2 => trm_while (aux t1) (aux t2)
+  | trm_for x t1 t2 t3 => trm_for x (aux t1) (aux t2) (subst (ctx_rem x E) t3)
   end.
+
+(** [subst1 z v t] replaces occurences of binder [z] with [v] in [t]. *)
+
+Definition subst1 (z:bind) (v:val) (t:trm) :=
+  subst (ctx_one z v) t.
+
+Definition subst2 (z1:bind) (v1:val) (z2:bind) (v2:val) (t:trm) :=
+  subst (ctx_two z1 v1 z2 v2) t.
 
 
 (* ---------------------------------------------------------------------- *)
 (** Big-step evaluation *)
-
-Section Red.
-
-Definition state := fmap loc val.
-
-Local Open Scope fmap_scope.
 
 Implicit Types t : trm.
 Implicit Types v : val.
@@ -195,8 +226,17 @@ Implicit Types l : loc.
 Implicit Types i : field.
 Implicit Types b : bool.
 Implicit Types n : int.
+Implicit Types x : var.
+Implicit Types z : bind.
+
+Definition state := fmap loc val.
+
+Section Red.
+
+Local Open Scope fmap_scope.
 
 Inductive red : state -> trm -> state -> val -> Prop :=
+  (* Core constructs *)
   | red_val : forall m v,
       red m v m v
   | red_fix : forall m f x t1,
@@ -205,24 +245,33 @@ Inductive red : state -> trm -> state -> val -> Prop :=
       red m1 t0 m2 (val_bool b) ->
       red m2 (if b then t1 else t2) m3 r ->
       red m1 (trm_if t0 t1 t2) m3 r
-  | red_let : forall m1 m2 m3 x t1 t2 v1 r,
+  | red_let : forall m1 m2 m3 z t1 t2 v1 r,
       red m1 t1 m2 v1 ->
-      red m2 (subst x v1 t2) m3 r ->
-      red m1 (trm_let x t1 t2) m3 r
-  | red_app_arg : forall m1 m2 m3 m4 t1 t2 v1 v2 r,
-      (~ trm_is_val t1 \/ ~ trm_is_val t2) ->
+      red m2 (subst1 z v1 t2) m3 r ->
+      red m1 (trm_let z t1 t2) m3 r
+  | red_app : forall m1 m2 m3 m4 t1 t2 f z t3 v1 v2 r,
       red m1 t1 m2 v1 ->
       red m2 t2 m3 v2 ->
-      red m3 (trm_app v1 v2) m4 r ->
+      v1 = val_fix f z t3 ->
+      red m3 (subst2 f v1 z v2 t3) m4 r ->
       red m1 (trm_app t1 t2) m4 r
-  | red_app_fun : forall m1 m2 v1 v2 x t r,
-      v1 = val_fun x t ->
-      red m1 (subst x v2 t) m2 r ->
-      red m1 (trm_app v1 v2) m2 r
-  | red_app_fix : forall m1 m2 v1 v2 f x t r,
-      v1 = val_fix f x t ->
-      red m1 (subst f v1 (subst x v2 t)) m2 r ->
-      red m1 (trm_app v1 v2) m2 r
+  | red_while : forall m1 m2 t1 t2 r,
+      red m1 (trm_if t1 (trm_seq t2 (trm_while t1 t2)) val_unit) m2 r ->
+      red m1 (trm_while t1 t2) m2 r
+  | red_for_arg : forall m1 m2 m3 m4 v1 v2 x t1 t2 t3 r,
+      (* LATER: add [not_is_val t1 \/ not_is_val t2] *)
+      red m1 t1 m2 v1 ->
+      red m2 t2 m3 v2 ->
+      red m3 (trm_for x v1 v2 t3) m4 r ->
+      red m1 (trm_for x t1 t2 t3) m4 r
+  | red_for : forall m1 m2 (x:var) n1 n2 t3 r,
+      red m1 (
+        If (n1 <= n2)
+          then (trm_seq (subst1 x n1 t3) (trm_for x (n1+1) n2 t3))
+          else val_unit) m2 r ->
+      red m1 (trm_for x n1 n2 t3) m2 r
+
+  (* Primitive operations on the heap *)
   | red_ref : forall ma mb v l,
       mb = (fmap_single l v) ->
       l <> null ->
@@ -240,6 +289,7 @@ Inductive red : state -> trm -> state -> val -> Prop :=
       l <> null ->
       \# ma mb ->
       red ma (val_alloc (val_int n)) (mb \+ ma) (val_loc l)
+  (* Other primitive operations *)
   | red_add : forall m n1 n2 n',
       n' = n1 + n2 ->
       red m (val_add (val_int n1) (val_int n2)) m (val_int n')
@@ -250,22 +300,7 @@ Inductive red : state -> trm -> state -> val -> Prop :=
       (l':nat) = (l:nat) + n :> int ->
       red m (val_ptr_add (val_loc l) (val_int n)) m (val_loc l')
   | red_eq : forall m v1 v2,
-      red m (val_eq v1 v2) m (val_bool (isTrue (v1 = v2)))
-  | red_while : forall m1 m2 t1 t2 r,
-      red m1 (trm_if t1 (trm_seq t2 (trm_while t1 t2)) val_unit) m2 r ->
-      red m1 (trm_while t1 t2) m2 r
-  | red_for_arg : forall m1 m2 m3 m4 v1 v2 x t1 t2 t3 r,
-      (* LATER: add [not_is_val t1 \/ not_is_val t2] *)
-      red m1 t1 m2 v1 ->
-      red m2 t2 m3 v2 ->
-      red m3 (trm_for x v1 v2 t3) m4 r ->
-      red m1 (trm_for x t1 t2 t3) m4 r
-  | red_for : forall m1 m2 x n1 n2 t3 r,
-      red m1 (
-        If (n1 <= n2)
-          then (trm_seq (subst x n1 t3) (trm_for x (n1+1) n2 t3))
-          else val_unit) m2 r ->
-      red m1 (trm_for x n1 n2 t3) m2 r.
+      red m (val_eq v1 v2) m (val_bool (isTrue (v1 = v2))).
 
   (* Remark: alternative for red_for rules.
     | red_for : forall m1 m2 m3 m4 v1 v2 x t1 t2 t3 r,
@@ -273,57 +308,210 @@ Inductive red : state -> trm -> state -> val -> Prop :=
           (trm_seq (trm_let x n1 t3) (trm_for x (n1+1) n2 t3))
           val_unit) m2 r ->
         red m1 (trm_for x n1 n2 t3) m2 r
+
+  Definition trm_is_val (t:trm) : Prop :=
+  match t with
+  | trm_val v => True
+  | _ => False
+  end.
+
   *)
 
-
-(* ---------------------------------------------------------------------- *)
-(* ** Properties of variable matching *)
-
-Lemma var_match_anon : forall x,
-  var_match x var_anon = false.
-Proof using. intros. destruct~ x. Qed.
-
-Lemma var_match_true_inv : forall x1 x2,
-  var_match x1 x2 = true ->
-  x1 = x2.
-Proof using. 
-  introv M. destruct x1; destruct x2; simpls; auto_false.
-  { rewrite name_eq_spec in M. rew_bool_eq in *. inverts* M. }
-Qed.
-
-Lemma var_match_false_inv : forall x1 x2,
-  var_match x1 x2 = false ->
-  x1 <> x2 \/ x1 = var_anon \/ x2 = var_anon.
-Proof using. 
-  introv M. destruct x1; destruct x2; simpls; auto_false.
-  { rewrite name_eq_spec in M. rew_bool_eq in *. left. intros E. inverts* E. }
-Qed.
+End Red.
 
 
 (* ---------------------------------------------------------------------- *)
-(* ** Properties of anonymous substitution *)
+(** Reintroduce contexts *)
 
-Lemma subst_anon : forall v t,
-  subst var_anon v t = t.
+Lemma nil_eq_ctx_empty : 
+  @nil (prod var val) = ctx_empty.
+Proof using. auto. Qed.
+
+Lemma cons_eq_ctx_add : forall x v (E:ctx),
+  (x,v)::E = ctx_add x v E.
+Proof using. auto. Qed.
+
+Hint Rewrite nil_eq_ctx_empty cons_eq_ctx_add : rew_ctx.
+
+Tactic Notation "rew_ctx" := 
+  autorewrite with rew_ctx.
+Tactic Notation "rew_ctx" "in" hyp(H) := 
+  autorewrite with rew_ctx in H.
+Tactic Notation "rew_ctx" "in" "*" := 
+  autorewrite with rew_ctx in *.
+
+
+(* ---------------------------------------------------------------------- *)
+(** Properties of operations on contexts  *)
+
+Lemma ctx_fresh_inv : forall (x1 x2:var) v E,
+  ctx_fresh x1 (ctx_add x2 v E) ->
+  x1 <> x2 /\ ctx_fresh x1 E.
+Proof using. 
+  introv M. unfolds ctx_fresh. simpls.
+  rewrite var_eq_spec in *. case_if~.
+Qed.
+
+(** [ctx_rem x ctx_empty] *)
+
+Lemma ctx_rem_empty : forall z,
+  ctx_rem z ctx_empty = ctx_empty.
+Proof using. intros. destruct z as [|x]; auto. Qed.
+
+(** Result of removing a variable from a context. *)
+(* -- TODO: rename and check useful *)
+
+Lemma ctx_rem_add_same : forall z v E,
+  ctx_rem z (ctx_add z v E) = ctx_rem z E.
+Proof using.
+  intros. destruct z as [|x].
+  { auto. }
+  { simpl. rewrite var_eq_spec. case_if~. }
+Qed.
+
+Lemma ctx_rem_add_neq : forall z1 z2 v E,
+  z1 <> z2 ->
+  ctx_rem z1 (ctx_add z2 v E) = ctx_add z2 v (ctx_rem z1 E).
+Proof using.
+  intros. destruct z2 as [|x2]. 
+  { auto. }
+  { destruct z1 as [|x1]. 
+    { auto. }
+    { simpl. rewrite var_eq_spec. case_if~. } }
+Qed.
+
+(** Removing a variable that does not occur in a context changes nothing. *)
+
+Lemma ctx_rem_fresh : forall x E,
+  ctx_fresh x E ->
+  ctx_rem x E = E.
+Proof using.
+  introv M. unfold ctx_rem. induction E as [|(y,v) E'].
+  { auto. }
+  { simpls. lets (N1&N2): ctx_fresh_inv (rm M).
+    rewrite var_eq_spec in *. case_if. rewrite~ IHE'. }
+Qed.
+
+(** [subst] with [ctx_empty] changes nothing. *)
+
+Lemma subst_ctx_empty : forall t,
+  subst ctx_empty t = t.
 Proof using.
   intros. induction t; simpl; 
-   try solve [ repeat rewrite var_match_anon; fequals ].
+   try solve [ repeat rewrite ctx_rem_empty; fequals* ].
+Qed.
+
+(** [subst1 z v t] when [z] is anonymous returns [t] unchanged. *)
+
+Lemma subst1_anon : forall v t,
+  subst1 bind_anon v t = t.
+Proof using.
+  intros. unfold subst1, ctx_one, ctx_add. rewrite~ subst_ctx_empty.
+Qed.
+
+Lemma ctx_rem_rem_neq : forall z1 z2 E,
+  ctx_rem z1 (ctx_rem z2 E) = ctx_rem z2 (ctx_rem z1 E).
+Proof using. (*
+
+  introv M. unfold ctx_rem. induction E as [|(y,v) E'].
+  { auto. }
+  { simpls. lets (N1&N2): ctx_fresh_inv (rm M).
+    rewrite var_eq_spec in *. case_if. rewrite~ IHE'. }
+*) admit.
+Qed.
+
+(** [subst] can be combuted  by iteratively substituting its bindings. *)
+
+Lemma subst_ctx_add : forall z v E t,
+  subst (ctx_add z v E) t = subst E (subst1 z v t).
+Proof using.
+  intros. destruct z as [|x].
+  { simpl. rewrite~ subst1_anon. }
+  { unfold subst1. simpl. rew_ctx. gen E. 
+    induction t; intros; simpl; try solve [ fequals* ].
+    { rewrite var_eq_spec. case_if~. }
+    { rew_ctx. fequals. tests: (b = x).
+      { repeat rewrite ctx_rem_add_same. fequals.
+        rewrite ctx_rem_empty, subst_ctx_empty. auto. }
+      { rewrite~ ctx_rem_add_neq. tests: (b0 = x).
+        { rewrite ctx_rem_add_same. fequals.
+          rewrite ctx_rem_rem_neq. rewrite ctx_rem_add_same.
+          rewrite ctx_rem_empty, subst_ctx_empty. auto. }
+        { do 3 rewrite~ ctx_rem_add_neq. do 2 rewrite ctx_rem_empty.
+          rewrite~ IHt. } } }
+  { rew_ctx. fequals. tests: (b = x).
+    { do 2 rewrite ctx_rem_add_same. fequals. rewrite~ subst_ctx_empty. }
+    { do 2 (rewrite~ ctx_rem_add_neq). rewrite ctx_rem_empty. rewrite~ IHt2. } }
+  { skip. (* todo *) } }
+Qed.
+
+Lemma subst1_subst_ctx_rem_same : forall E x v t,
+    subst1 x v (subst (ctx_rem x E) t)
+  = subst E (subst1 x v t).
+Proof using.
+  intros. rewrite <- subst_ctx_add.
+(* 
+  intros E. induction E as [|(y,w) E']; simpl; intros.
+  { auto. }
+  { rewrite var_eq_spec. case_if.
+    { subst. rewrite IHE'. rewrite~ subst_subst_same. }
+    { simpl. rewrite IHE'. rewrite~ subst_subst_neq. } }
+Qed.
+*)
+Admitted.
+
+Lemma subst1_subst : forall x v E t,
+  ctx_fresh x E ->
+  subst1 x v (subst E t) = subst E (subst1 x v t).
+Proof using.
+  introv M. rewrite <- (@subst1_subst_ctx_rem_same E x v t).
+  fequals. rewrite~ ctx_rem_fresh.
 Qed.
 
 
+(*
+
+  (** Substituting for [E] without [x] then substituting for [x]
+      is equivalent to substituting for [x] then for [E]
+      (even if [x] is bound in [E]). *)
+
+
+  (** Substitutions for two distinct variables commute. *)
+
+  Lemma subst1_subst1_neq : forall x1 x2 v1 v2 t,
+    x1 <> x2 ->
+    subst1 x2 v2 (subst1 x1 v1 t) = subst1 x1 v1 (subst1 x2 v2 t).
+  Proof using.
+    introv N. induction t; simpl; try solve [ fequals;
+    repeat case_if; simpl; repeat case_if; auto ].
+    repeat case_if; simpl; repeat case_if~.
+    { false. destruct v; destruct x1; destruct x2; false. simpls.
+      rewrite name_eq_spec in *. rew_bool_eq in *. false. }
+  Qed. (* LATER: simplify *)
+
+  (** Substituting for a variable that has just been substituted
+      does not further modify the term. *)
+
+  Lemma subst_subst_same : forall x v1 v2 t,
+    subst1 x v2 (subst1 x v1 t) = subst1 x v1 t.
+  Proof using.
+    intros. induction t; simpl; try solve [ fequals;
+    repeat case_if; simpl; repeat case_if; auto ].
+  Qed.
+*)
 
 (* ---------------------------------------------------------------------- *)
 (* ** Derived rules *)
 
 Lemma red_fun : forall m x t1,
   red m (trm_fun x t1) m (val_fun x t1).
-Proof using. intros. applys red_fix. Qed.
+Proof using. intros. apply red_fix. Qed.
 
 Lemma red_seq : forall m1 m2 m3 t1 t2 r1 r,
   red m1 t1 m2 r1 ->
   red m2 t2 m3 r ->
   red m1 (trm_seq t1 t2) m3 r.
-Proof using. introv M1 M2. applys* red_let. rewrite* subst_anon. Qed.
+Proof using. introv M1 M2. applys* red_let. rewrite* subst1_anon. Qed.
 
 Lemma red_ptr_add_nat : forall m l (f : nat),
   red m (val_ptr_add (val_loc l) (val_int f)) m (val_loc (l+f)%nat).
@@ -336,7 +524,7 @@ Proof using. introv M1. applys* red_if. applys red_val. Qed.
 
 Lemma red_for_le : forall m1 m2 m3 x n1 n2 t3 r,
   n1 <= n2 ->
-  red m1 (subst x n1 t3) m2 val_unit ->
+  red m1 (subst1 x n1 t3) m2 val_unit ->
   red m2 (trm_for x (n1+1) n2 t3) m3 r ->
   red m1 (trm_for x n1 n2 t3) m3 r.
 Proof using.
@@ -354,7 +542,7 @@ Proof using.
   { applys red_val. }
 Qed.
 
-End Red.
+
 
 
 (* ********************************************************************** *)
@@ -478,6 +666,8 @@ Open Scope var_scope.
 
 (* ---------------------------------------------------------------------- *)
 (** Notation for concrete programs *)
+
+(* TODO: rename some x into z *)
 
 Notation "'()" := val_unit : trm_scope.
 
@@ -630,32 +820,6 @@ Notation "t1 '= t2" :=
 (* ********************************************************************** *)
 (* * More on substitutions *)
 
-(* ---------------------------------------------------------------------- *)
-(** Properties of substitution *)
-
-(** Substitutions for two distinct variables commute. *)
-
-Lemma subst_subst_neq : forall x1 x2 v1 v2 t,
-  x1 <> x2 ->
-  subst x2 v2 (subst x1 v1 t) = subst x1 v1 (subst x2 v2 t).
-Proof using.
-  introv N. induction t; simpl; try solve [ fequals;
-  repeat case_if; simpl; repeat case_if; auto ].
-  repeat case_if; simpl; repeat case_if~.
-  { false. destruct v; destruct x1; destruct x2; false. simpls.
-    rewrite name_eq_spec in *. rew_bool_eq in *. false. }
-Qed. (* LATER: simplify *)
-
-(** Substituting for a variable that has just been substituted
-    does not further modify the term. *)
-
-Lemma subst_subst_same : forall x v1 v2 t,
-  subst x v2 (subst x v1 t) = subst x v1 t.
-Proof using.
-  intros. induction t; simpl; try solve [ fequals;
-  repeat case_if; simpl; repeat case_if; auto ].
-Qed.
-
 
 (* ---------------------------------------------------------------------- *)
 (** Distinct variables *)
@@ -682,237 +846,29 @@ Fixpoint var_distinct (xs:vars) : bool :=
 
 
 (* ---------------------------------------------------------------------- *)
-(** Iterated substitution *)
-
-(** [ctx] describes a list of bindings *)
-
-Definition ctx := list (var*val).
-
-(** [ctx_empty] describes the empty context *)
-
-Definition ctx_empty : ctx :=
-  nil.
-
-(** [ctx_add x v E] extends [E] with a binding from [x] to [v] *)
-
-Definition ctx_add (x:var) (v:val) (E:ctx) :=
-  (x,v)::E.
-
-(** [ctx_rem x E] removes all bindings on [x] stored in [E] *)
-
-Fixpoint ctx_rem (x:var) (E:ctx) : ctx :=
-  match E with
-  | nil => nil
-  | (y,v)::E' =>
-    let E'' := ctx_rem x E' in
-    if var_eq x y then E'' else (y,v)::E''
-  end.
-
-(** [ctx_lookup x E] returns
-    - [None] if [x] is not bound in [E]
-    - [Some v] if [x] is bound to [v] in [E]. *)
-
-Fixpoint ctx_lookup (x:var) (E:ctx) : option val :=
-  match E with
-  | nil => None
-  | (y,v)::E' => if var_match x y
-                   then Some v
-                   else ctx_lookup x E'
-  end.
-
-(** [ctx_fresh x E] asserts that [x] is not bound in [E] *)
-
-Fixpoint ctx_fresh (x:var) (E:ctx) : bool :=
-  match E with
-  | nil => true
-  | (y,v)::E' => if var_eq x y then false else ctx_fresh x E'
-  end.
-
-(* todo: deprecated
-Definition ctx_fresh (x:var) (E:ctx) : Prop :=
-  ctx_lookup x E = None.
-*)
-
-(** [substs E t] substitutes all the bindings from [E] inside [t] *)
-
-Fixpoint substs (E:ctx) (t:trm) :=
-  match E with
-  | nil => t
-  | (x,v)::E' => substs E' (subst x v t)
-  end.
-
-
-(* ---------------------------------------------------------------------- *)
-(** Properties of iterated substitution *)
-
-(** Simplification equalities for [ctx_rem] *)
-
-Lemma ctx_rem_same : forall x v E,
-  ctx_rem x ((x,v)::E) = ctx_rem x E.
-Proof using. intros. simpl. rewrite var_eq_spec. case_if~. Qed.
-
-Lemma ctx_rem_neq : forall x y v E,
-  x <> y ->
-  ctx_rem x ((y,v)::E) = (y,v)::(ctx_rem x E).
-Proof using. intros. simpl. rewrite var_eq_spec. case_if~. Qed.
-
-(** Auxiliary results *)
-
-Lemma ctx_rem_fresh : forall x E,
-  ctx_fresh x E ->
-  ctx_rem x E = E.
-Proof using.
-  introv M. induction E as [|(y,v) E'].
-  { auto. } 
-  { simpls. rewrite var_eq_spec in *. case_if. fequals. rewrite~ IHE'. }
-Qed.
-
-(** Substituting for [E] without [x] then substituting for [x]
-    is equivalent to substituting for [x] then for [E]
-    (even if [x] is bound in [E]). *)
-
-Lemma subst_substs_ctx_rem_same : forall E x v t,
-    subst x v (substs (ctx_rem x E) t)
-  = substs E (subst x v t).
-Proof using.
-  intros E. induction E as [|(y,w) E']; simpl; intros.
-  { auto. }
-  { rewrite var_eq_spec. case_if.
-    { subst. rewrite IHE'. rewrite~ subst_subst_same. }
-    { simpl. rewrite IHE'. rewrite~ subst_subst_neq. } }
-Qed.
-
-Lemma subst_substs : forall x v E t,
-  ctx_fresh x E ->
-  subst x v (substs E t) = substs E (subst x v t).
-Proof using.
-  introv M. forwards N: subst_substs_ctx_rem_same E x v t.
-  rewrite~ ctx_rem_fresh in N.
-Qed.
-
-(** The following lemmas describe how iterated substitution
-    distributes over the construction of the language *)
-
-Ltac substs_simpl_proof :=
-  let x := fresh "x" in let w := fresh "w" in
-  let E := fresh "E" in let E' := fresh "E'" in
-  let IH := fresh "IH" in
-  intros E; induction E as [|(x,w) E' IH]; intros; simpl;
-  [ | try rewrite IH ]; auto.
-
-Lemma substs_val : forall E v,
-  substs E (trm_val v) = v.
-Proof using. substs_simpl_proof. Qed.
-
-Lemma substs_var : forall E x,
-    substs E (trm_var x)
-  = match ctx_lookup x E with
-    | None => trm_var x
-    | Some v => v end.
-Proof using.
-  substs_simpl_proof.
-  { case_if.
-    { rewrite~ substs_val. }
-    { auto. } }
-Qed.
-
-Lemma substs_fun : forall E x t,
-  substs E (trm_fun x t) = trm_fun x (substs (ctx_rem x E) t).
-Proof using. 
-  substs_simpl_proof. 
-  { fequals. rewrite var_eq_spec.
-    case_eq (var_match x0 x); introv M.
-    { lets: var_match_true_inv M. subst. case_if~. }
-    { lets [N|[N|N]]: var_match_false_inv M.
-      { case_if~. }
-      { case_if~. subst. rewrite~ subst_anon. }
-      { case_if~. subst. rewrite~ subst_anon. } } }
-Qed.
-
-Lemma substs_fix : forall E f x t,
-  substs E (trm_fix f x t) = trm_fix f x (substs (ctx_rem x (ctx_rem f E)) t).
-Proof using.
-  substs_simpl_proof.
-  { fequals. rewrite var_eq_spec.
-    case_eq (var_match f x); introv M1.
-    { lets: var_match_true_inv M1. subst. case_if~. }
-    { lets [N1|[N1|N1]]: var_match_false_inv M1.
-      { case_eq (var_match x0 x); introv M2.
-        { lets: var_match_true_inv M2. subst. case_if~. rewrite~ ctx_rem_same. }
-        { lets [N2|[N2|N2]]: var_match_false_inv M2.
-          { case_if. { rewrite~ ctx_rem_neq. } }
-          { subst. case_if~. admit. (*todo *) } 
-          { subst. case_if~. rewrite subst_anon. (* todo: same as later *) admit. } } }
-      { subst. case_eq (var_match x0 x); introv M2.
-        { lets: var_match_true_inv M2. subst. case_if~. rewrite~ ctx_rem_same. }
-        { lets [N2|[N2|N2]]: var_match_false_inv M2.
-          { case_if. { subst. rewrite~ subst_anon. } { rewrite~ ctx_rem_neq. } }
-          { subst. case_if~.
-            { subst. rewrite~ subst_anon. } 
-            { rewrite~ ctx_rem_neq. } } 
-          { subst. case_if~.
-            { subst. rewrite~ subst_anon. } } } }
-      { subst. rewrite var_match_anon. rewrite subst_anon.
-        case_if~.  (* todo: substs  with var_anon  in ctx  is irrelevant *) admit. } } }
-Qed.
-
-Lemma substs_if : forall E t1 t2 t3,
-   substs E (trm_if t1 t2 t3)
- = trm_if (substs E t1) (substs E t2) (substs E t3).
-Proof using. substs_simpl_proof. Qed.
-
-Lemma substs_app : forall E t1 t2,
-   substs E (trm_app t1 t2)
- = trm_app (substs E t1) (substs E t2).
-Proof using. substs_simpl_proof. Qed.
-
-Lemma substs_seq : forall E t1 t2,
-   substs E (trm_seq t1 t2)
- = trm_seq (substs E t1) (substs E t2).
-Proof using. substs_simpl_proof. Qed.
-
-Lemma substs_let : forall E x t1 t2,
-   substs E (trm_let x t1 t2)
- = trm_let x (substs E t1) (substs (ctx_rem x E) t2).
-Proof using. substs_simpl_proof. { fequals. case_if~. } Qed.
-
-Lemma substs_while : forall E t1 t2,
-   substs E (trm_while t1 t2)
- = trm_while (substs E t1) (substs E t2).
-Proof using. substs_simpl_proof. Qed.
-
-
-
-(* ---------------------------------------------------------------------- *)
 (** N-ary substitution *)
 
-(** Shorthand [names], [vals] and [trms] for lists of items. *)
+(** Shorthand [vars], [vals] and [trms] for lists of items. *)
 
-Definition names := list name.
 Definition vals : Type := list val.
 Definition trms : Type := list trm.
-
-(** Coercion from list of names to list of variables *)
-
-Coercion names_to_vars (xs:names) :=
-  List.map var_name xs.
 
 (** [substn xs vs t] is a shorthand for [substs (List.combine xs vs) t].
     It substitutes the values [vs] for the corresponding variables in [xs].
     This operation is only specified when [length xs = length vs]. *)
 
 Definition substn (xs:vars) (vs:vals) (t:trm) : trm :=
-  substs (LibList.combine xs vs) t.
+  subst (LibList.combine xs vs) t.
 
 (** Distribution of [substn] on [nil] and [cons] lists *)
 
 Lemma substn_nil : forall t,
   substn nil nil t = t.
-Proof using. auto. Qed.
+Proof using. intros. unfold substn. simpl. rew_ctx. apply subst_ctx_empty. Qed.
 
 Lemma substn_cons : forall x xs v vs t,
-  substn (x::xs) (v::vs) t = substn xs vs (subst x v t).
-Proof using. auto. Qed.
+  substn (x::xs) (v::vs) t = substn xs vs (subst1 x v t).
+Proof using. intros. unfold substn. simpl. rew_ctx. rewrite~ subst_ctx_add. Qed.
 
 (** Auxiliary results for freshness of bindings w.r.t. combine *)
 
@@ -925,7 +881,7 @@ Proof using.
   induction ys as [|y ys']; simpl; intros [|v vs] M L;
    rew_list in *; try solve [ false; math ].
   { auto. }
-  { simpl. do 2 case_if. rewrite~ IHys'. }
+  { simpl. rewrite var_eq_spec in *. do 2 case_if. rewrite~ IHys'. }
 Qed.
 
 (* Permutation lemma for substitution and n-ary substitution *)
@@ -933,9 +889,9 @@ Qed.
 Lemma subst_substn : forall x v ys ws t,
   var_fresh x ys ->
   length ys = length ws ->
-  subst x v (substn ys ws t) = substn ys ws (subst x v t).
+  subst1 x v (substn ys ws t) = substn ys ws (subst1 x v t).
 Proof using.
-  introv M L. unfold substn. rewrite~ subst_substs.
+  introv M L. unfold substn. rewrite~ subst1_subst.
   applys~ ctx_fresh_combine.
 Qed.
 
@@ -992,29 +948,23 @@ Fixpoint trm_apps (tf:trm) (ts:trms) : trm :=
   | t::ts' => trm_apps (trm_app tf t) ts'
   end.
 
-Fixpoint trm_funs (xs:vars) (t:trm) : trm :=
+Fixpoint trm_fixs (f:bind) (xs:vars) (t:trm) : trm :=
   match xs with
   | nil => t
-  | x::xs' => trm_fun x (trm_funs xs' t)
+  | x::xs' => trm_fix f x (trm_fixs bind_anon xs' t)
   end.
 
-Definition val_funs (xs:vars) (t:trm) : val :=
+Definition val_fixs (f:bind) (xs:vars) (t:trm) : val :=
   match xs with
   | nil => arbitrary
-  | x::xs' => val_fun x (trm_funs xs' t)
+  | x::xs' => val_fix f x (trm_fixs bind_anon xs' t)
   end.
 
-Definition trm_fixs (f:var) (xs:vars) (t:trm) : trm :=
-  match xs with
-  | nil => t
-  | x::xs' => trm_fix f x (trm_funs xs' t)
-  end.
+Notation "'trm_funs' xs t1" := (trm_fixs bind_anon xs t1)
+  (at level 69, xs at level 0, t1 at level 0).
 
-Definition val_fixs (f:var) (xs:vars) (t:trm) : val :=
-  match xs with
-  | nil => arbitrary
-  | x::xs' => val_fix f x (trm_funs xs' t)
-  end.
+Notation "'val_funs' xs t1" := (val_fixs bind_anon xs t1)
+  (at level 69, xs at level 0, t1 at level 0).
 
 
 (* ---------------------------------------------------------------------- *)
@@ -1033,7 +983,7 @@ Definition var_funs_exec (n:nat) (xs:vars) : bool :=
   && is_not_nil xs
   && var_distinct xs.
 
-Lemma var_funs_exec_eq : forall n xs,
+Lemma var_funs_exec_eq : forall (n:nat) xs,
   var_funs_exec n xs = isTrue (var_funs n xs).
 Proof using.
   intros. unfold var_funs_exec, var_funs.
@@ -1053,7 +1003,7 @@ Definition var_fixs_exec (f:var) (n:nat) (xs:vars) : bool :=
   && is_not_nil xs
   && var_distinct (f::xs).
 
-Lemma var_fixs_exec_eq : forall f n xs,
+Lemma var_fixs_exec_eq : forall f (n:nat) xs,
   var_fixs_exec f n xs = isTrue (var_fixs f n xs).
 Proof using.
   intros. unfold var_fixs_exec, var_fixs.
@@ -1077,10 +1027,10 @@ Qed.
 
 Lemma subst_trm_funs : forall y w xs t,
   var_fresh y xs ->
-  subst y w (trm_funs xs t) = trm_funs xs (subst y w t).
+  subst1 y w (trm_funs xs t) = trm_funs xs (subst1 y w t).
 Proof using.
-  introv N. induction xs as [|x xs']; simpls; fequals.
-  { case_if. rewrite~ IHxs'. }
+  introv N. unfold subst1. induction xs as [|x xs']; simpls; fequals.
+  { rewrite var_eq_spec in *. case_if. rewrite~ <- IHxs'. }
 Qed.
 
 Lemma red_app_funs_val_ind : forall xs vs m1 m2 tf t r,
@@ -1096,10 +1046,11 @@ Proof using.
     simpls. tests C: (xs' = nil).
     { rew_list in *. asserts: (vs' = nil).
       { applys length_zero_inv. math. } subst vs'. clear L.
-      simpls. applys~ red_app_arg R. applys~ red_app_fun. }
-    { rew_istrue in N. destruct N as [F N']. applys~ IHxs' M.
-      applys~ red_app_arg R. applys~ red_app_fun.
-      rewrite~ subst_trm_funs. applys~ red_funs. splits~. } }
+      simpls. applys* red_app. }
+    { rew_istrue in N. destruct N as [F N'].
+      unfold substn in M. simpl combine in M. rew_ctx in M. 
+      rewrite subst_ctx_add in M. applys~ IHxs' M. applys* red_app.
+      { rewrite~ subst_trm_funs. applys~ red_funs. } { splits~. } } }
 Qed.
 
 Lemma red_app_funs_val : forall xs vs m1 m2 vf t r,
@@ -1114,7 +1065,7 @@ Qed.
 
 
 (* ---------------------------------------------------------------------- *)
-(** Properties of n-ary recursive functions *)
+(** Properties of n-ary functions *)
 
 Lemma red_fixs : forall m f xs t,
   xs <> nil ->
@@ -1126,16 +1077,21 @@ Qed.
 
 Lemma subst_trm_fixs : forall y w f xs t,
   var_fresh y (f::xs) ->
-  subst y w (trm_fixs f xs t) = trm_fixs f xs (subst y w t).
+  subst1 y w (trm_fixs f xs t) = trm_fixs f xs (subst1 y w t).
 Proof using.
-  introv N. unfold trm_fixs. destruct xs as [|x xs'].
+  introv N. destruct xs as [|x xs'].
   { auto. }
-  { simpls. do 2 case_if in N. rewrite~ subst_trm_funs. }
-Qed.
+  { unfold subst1. simpls. repeat rewrite var_eq_spec in *.
+    do 2 case_if in N. simpl. rewrite var_eq_spec. case_if~.
+    fequals. 
+    forwards K: subst_trm_funs N. unfold subst1, ctx_one in K.
+    simpls. rewrite~ K. }
+Qed.  (* LATER: simplify *) 
 
-Lemma red_app_fixs_val : forall xs vs m1 m2 vf f t r,
+(* LATER
+Lemma red_app_fixs_val : forall xs vs m1 m2 vf (f:var) t r,
   vf = val_fixs f xs t ->
-  red m1 (subst f vf (substn xs vs t)) m2 r ->
+  red m1 (subst1 f vf (substn xs vs t)) m2 r ->
   var_fixs f (length vs) xs ->
   red m1 (trm_apps vf vs) m2 r.
 Proof using.
@@ -1145,14 +1101,14 @@ Proof using.
     tests C':(xs' = nil).
     { rew_list in *. asserts: (vs' = nil).
       { applys length_zero_inv. math. } subst vs'. clear L.
-      simpls. applys* red_app_fix. }
+      simpls. applys* red_app. }
     { applys~ red_app_funs_val_ind.
       { applys* red_app_fix. do 2 rewrite~ subst_trm_funs. applys~ red_funs. }
       { rewrite~ subst_substn in M. { rewrite~ substn_cons in M.
         rewrite~ subst_subst_neq. } { simpl. case_if~. } }
       { splits*. } } }
 Qed.
-
+*)
 
 (* ---------------------------------------------------------------------- *)
 (** Folding of n-ary functions *)
@@ -1241,31 +1197,34 @@ Tactic Notation "rew_nary" "in" "*" :=
   (* rewrite_strat (any (innermost (hints rew_nary))).
      => way too slow! *)
 
-Lemma rew_nary_demo_1 : forall f x y z t1 t2 t,
+(* todo fix
+
+Lemma rew_nary_demo_1 : forall (f x y z:var) t1 t2 t,
   val_fix f x (trm_fun y (trm_fun z (f t1 x y t2))) = t.
 Proof using. intros. rew_nary. Abort.
 
 Lemma rew_nary_demo_2 : forall f x y t,
   val_fun f (trm_fun x (trm_fun y (x y))) = t.
 Proof using. intros. rew_nary. Abort.
+*)
 
 
 (* ---------------------------------------------------------------------- *)
 (* ** Sequence of consecutive variables *)
 
-(** [nat_to_name n] converts [nat] values into distinct
+(** [nat_to_var n] converts [nat] values into distinct
     [name] values.
     Warning: the current implementation is inefficient. *)
 
 Definition dummy_char := Ascii.ascii_of_nat 0%nat.
 
-Fixpoint nat_to_name (n:nat) : name :=
+Fixpoint nat_to_var (n:nat) : var :=
   match n with
   | O => String.EmptyString
-  | S n' => String.String dummy_char (nat_to_name n')
+  | S n' => String.String dummy_char (nat_to_var n')
   end.
 
-Lemma injective_nat_to_name : injective nat_to_name.
+Lemma injective_nat_to_var : injective nat_to_var.
 Proof using.
   intros n. induction n as [|n']; intros m E; destruct m as [|m']; tryfalse.
   { auto. }
@@ -1279,31 +1238,31 @@ Qed.
 Fixpoint var_seq (start:nat) (nb:nat) : vars :=
   match nb with
   | O => nil
-  | S nb' => (var_name (nat_to_name start)) :: var_seq (S start) nb'
+  | S nb' => (nat_to_var start) :: var_seq (S start) nb'
   end.
 
 Section Var_seq.
 Implicit Types start nb : nat.
 
-Lemma var_fresh_var_seq_lt : forall x start nb,
+Lemma var_fresh_var_seq_lt : forall (x:nat) start nb,
   (x < start)%nat ->
-  var_fresh (nat_to_name x) (var_seq start nb).
+  var_fresh (nat_to_var x) (var_seq start nb).
 Proof using.
   intros. gen start. induction nb; intros.
   { auto. }
-  { simpl. case_if.
-    { lets: injective_nat_to_name C. math. }
+  { simpl. rewrite var_eq_spec. case_if.
+    { lets: injective_nat_to_var C. math. }
     { applys IHnb. math. } }
 Qed.
 
-Lemma var_fresh_var_seq_ge : forall x start nb,
+Lemma var_fresh_var_seq_ge : forall (x:nat) start nb,
   (x >= start+nb)%nat ->
-  var_fresh (nat_to_name x) (var_seq start nb).
+  var_fresh (nat_to_var x) (var_seq start nb).
 Proof using.
   intros. gen start. induction nb; intros.
   { auto. }
-  { simpl. case_if.
-    { lets: injective_nat_to_name C. math. }
+  { simpl. rewrite var_eq_spec. case_if.
+    { lets: injective_nat_to_var C. math. }
     { applys IHnb. math. } }
 Qed.
 
